src/rocq/Theory/I2F_instr.v
@@ -1,0 +1,164 @@
+From Equations Require Import Equations.
+
+From Stdlib Require Import Lia.
+
+From ExtLib Require Import Structures.Monads.
+
+From ITree Require Import ITree Eq HeterogeneousRelations.
+
+From Vellvm Require Import
+  Utils
+  Syntax
+  VellvmIntegers
+  Integers
+  DynamicValues
+  EOU
+  LLVMEvents
+  Semantics.Operations
+  Interfaces.IPtr
+  Interfaces.Params
+  Implementations.Address
+  Implementations.Provenance
+  Implementations.IPtrInfinite
+  Implementations.IPtrFinite
+  Implementations.Memory
+  Implementations.ParamsV
+  Denotation.
+
+From Vellvm Require Import
+  Theory.rutt_cutoff
+  Theory.I2F.
+
+From Paco Require Import paco.
+  Ltac rstep :=
+    first [apply ruttc_trigger |
+            apply ruttc_trigger_cast |
+            apply ruttc_ret 
+      ].
+
+Tactic Notation "rbind" uconstr(x) := eapply ruttc_bind with (RR := x).
+Tactic Notation "erbind" := eapply ruttc_bind.
+
+From Stdlib Require Import
+  Program Setoid Morphisms List.
+
+#[global]Instance ruttc_eq_itree {E1 E2 R1 R2 Rcutr Rcutl REv RAns RR} :
+  Proper (eq_itree Logic.eq ==> eq_itree Logic.eq ==> flip impl) (@ruttc E1 E2 R1 R2 Rcutr Rcutl REv RAns RR).
+Proof.
+  intros ?? EQ1 ?? EQ2; rewrite EQ1,EQ2; intuition.
+Qed.
+
+Ltac cbnn := cbn; unfold resum, ReSum_id, id_, Id_IFun.
+Ltac bind_exp := erbind; [apply I2F_denote_exp'| intros].
+
+Lemma I2F_freeze' a b :
+  I2F_dvalue a b ->
+  I2F_refine_CFG I2F_dvalue (freeze a) (freeze b).
+Proof with try now (rstep; cbnn; try (easy); eauto).
+  (* automation is different in this file from the expression one, to understand *)
+(*   intros HDV. *)
+(*   induction HDV; cbn... *)
+
+(*   all: eapply ruttc_bind; [apply ruttc_map_monad_gen; eauto |]; intros... *)
+(* Qed.  *)
+Admitted.
+
+Lemma I2F_denote_instr :
+  forall i va1 va2,
+    option_rel I2F_Addr va1 va2 ->
+      I2F_refine_CFG TT
+        (@denote_instr PInf i va1) (@denote_instr PFin i va2).
+  Proof with try now (rstep; cbnn; try (easy); eauto).
+    intros [[x i] ?] ? ? HR.
+    destruct i.
+    - cbn; break_match...
+    - cbn; break_match...
+      subst.
+      bind_exp.
+      rbind TT...
+      intros ???...
+    - destruct x, fn.
+      + cbn.
+        rbind (Forall2 I2F_dvalue).
+        { apply ruttc_map_monad.
+          intros [] HIN.
+          apply I2F_denote_exp'.
+        }
+        break_match...
+        * intros.
+          rewrite 2 Eqit.bind_bind.
+          rbind (sum_rel I2F_dvalue I2F_dvalue)...
+          intros * HR'.
+          inv HR'.
+          rbind (fun _ _ => False)...
+          intros ?? [].
+          rewrite 2 Eqit.bind_ret_l...
+        * intros.
+          rewrite 2 Eqit.bind_bind.
+          bind_exp.
+          rewrite 2 Eqit.bind_bind.
+          rbind (sum_rel I2F_dvalue I2F_dvalue)...
+          intros * HR'.
+          inv HR'.
+          rbind (fun _ _ => False)...
+          intros ?? [].
+          rewrite 2 Eqit.bind_ret_l...
+      + cbn.
+        rbind (Forall2 I2F_dvalue).
+        { apply ruttc_map_monad.
+          intros [] HIN.
+          apply I2F_denote_exp'.
+        }
+        intros.
+        break_match...
+        * intros.
+          rewrite 2 Eqit.bind_bind.
+          rbind (sum_rel I2F_dvalue I2F_dvalue)...
+          intros * HR'.
+          inv HR'.
+          rbind (fun _ _ => False)...
+          intros ?? [].
+          rewrite 2 Eqit.bind_ret_l...
+        * intros.
+          rewrite 2 Eqit.bind_bind.
+          bind_exp.
+          rewrite 2 Eqit.bind_bind.
+          rbind (sum_rel I2F_dvalue I2F_dvalue)...
+          intros * HR'.
+          inv HR'.
+          rbind (fun _ _ => False)...
+          intros ?? [].
+          rewrite 2 Eqit.bind_ret_l...
+        
+    - destruct x; cbn[denote_instr].
+      2: rstep; constructor.
+      admit.
+      (* break_match_goal. *)
+      (* + break_goal_fast. *)
+      (*   cbn. rewrite 2 Eqit.bind_bind. *)
+      (*   erbind; [apply I2F_denote_exp'| intros; rewrite ?Eqit.bind_bind]. *)
+      (*   rbind I2F_dvalue. *)
+      (*   { apply ruttc_trigger. *)
+      (*     constructor; intuition. *)
+      (*     2:{ cbn; intros... *)
+      (*     admit. *)
+      (*     (* cbn in *; unfold resum, ReSum_id, id_, Id_IFun. *) *)
+      (*     (* intros ??; rewrite I2FA_Memory_equation_13. *) *)
+      (*       (* in H0 *) *)
+    - destruct x; cbn...
+      destruct ptr.
+      bind_exp.
+      erbind; [rstep; [cbnn; easy |] |].
+      cbnn; intros; simp I2FA_Memory in *; eauto.
+      intros.
+      erbind; [apply I2F_freeze'; auto | intros]...
+    - destruct val,ptr, x; cbn...
+      bind_exp.
+      bind_exp.
+      induction H0...
+      6: rbind (fun _ _ => False); [|intros _ _ []]...
+      all: rbind (fun _ _ => True); [rstep; cbnn; [constructor; intuition; constructor; auto| cbn; auto] | intros [] [] _ ]; cbn...
+    -   
+     
+  Admitted.
+ 
